refactoring

src/theory/bir/bir_promising_diamondScript.sml
@@ -3,6 +3,7 @@ open bir_promisingTheory;
 open bir_programTheory;
 open bir_valuesTheory;
 open bir_expTheory;
+open bir_promising_wfTheory;
 open finite_mapTheory;
 
 val _ = new_theory "bir_promising_diamond";
@@ -16,508 +17,6 @@ Definition bir_nonpromise_step_def:
   nonpromise_step cid (cores,M) (cores',M') =
   (parstep cid cores M cores' M' /\ (M = M'))
 End
-
-Definition latest_def:
-  latest l 0 M = 0
-  /\ latest l (SUC t) M =
-  case oEL t M of
-    SOME msg =>
-      if l = msg.loc then SUC t else latest l t M
-  | _ => latest l t M
-End
-
-Definition well_formed_fwdb_def:
- well_formed_fwdb l M coh_t fwd =
-   (fwd.fwdb_time <= latest l coh_t M
-    /\ fwd.fwdb_view <= fwd.fwdb_time
-    /\ ?v. mem_read M l fwd.fwdb_time = SOME v)
-End
-(*
-Definition well_formed_xclb_def:
-  well_formed_xclb M coh_t xclb =
-  (xclb.xclb_time <= latest xclb.xclb_loc coh_t M
-   /\ xclb.xclb_view <= coh_t
-   /\ ?v. mem_read M xclb.xclb_loc xclb.xclb_time = SOME v)
-End
-*)
-
-Definition well_formed_viewenv_def:
-  well_formed_viewenv viewenv M =
-  !var v. FLOOKUP viewenv var = SOME v
-  ==>
-  v <= LENGTH M
-End
-
-Definition well_formed_def:
-  well_formed cid M s =
-  ( well_formed_viewenv s.bst_viewenv M
-    /\ (!l. s.bst_coh(l) <= LENGTH M)
-     /\ s.bst_v_rNew <= LENGTH M
-     /\ s.bst_v_rOld <= LENGTH M
-     /\ s.bst_v_wNew <= LENGTH M
-     /\ s.bst_v_wOld <= LENGTH M
-     /\ s.bst_v_CAP <= LENGTH M
-     /\ s.bst_v_Rel <= LENGTH M
-     /\ (!l. well_formed_fwdb l M (s.bst_coh(l)) (s.bst_fwdb(l)))
-(*     /\ (!xclb. s.bst_xclb = SOME xclb ==> well_formed_xclb M (s.bst_coh(xclb.loc) xclb)) *)
-     /\ (!t. MEM t s.bst_prom ==> t <= LENGTH M)
-     /\ (!t msg.
-           (oEL t M = SOME msg
-            /\ msg.cid = cid
-            /\ s.bst_coh(msg.loc) < t)
-           ==>
-           MEM t s.bst_prom)
-    )
-End
-
-Triviality mem_get_SOME:
-  !l t M msg.
-    mem_get M l t = SOME msg
-    ==>
-    l = msg.loc
-Proof
-  Cases_on ‘t’
-  >> fs[mem_get_def, mem_default_def]
-  >> rpt strip_tac
-  >> Cases_on ‘oEL n M’
-  >> gvs[]
-QED
-
-Theorem mem_get_mem_read:
-  !M l t v.
-    mem_read M l t = SOME v
-    ==>
-    ?m. mem_get M l t = SOME m /\ m.val = v
-Proof
-  Induct_on ‘t’ >- fs[mem_read_def, mem_get_def]
-  >> rpt strip_tac
-  >> fs[mem_read_def, mem_get_def]
-  >> Cases_on ‘oEL t M’
-  >- fs[]
-  >> Cases_on ‘x.loc = l’ >- fs[]
-  >> fs[]
-QED
-
-Theorem mem_get_append:
-  !t M l msg.
-    t <= LENGTH M ==> mem_get (M++[msg]) l t = mem_get M l t
-Proof
-  rpt strip_tac
-  >> Cases_on ‘t’
-  >> fs[mem_get_def] (* discharges 0 case, SUC remains *)
-  >> fs[listTheory.oEL_THM, rich_listTheory.EL_APPEND1]
-QED
-
-Triviality mem_read_some:
-  !M l t v.
-    mem_read M l t = SOME v ==> t <= LENGTH M \/ (t = 0 /\ v = mem_default_value)
-Proof
-  Induct_on ‘t’
-  >> rpt strip_tac
-  >> fs[mem_read_def,mem_get_def]
-  >> Cases_on ‘oEL t M’
-  >> fs[listTheory.oEL_EQ_EL, listTheory.oEL_def]
-QED
-
-Theorem programs_unchanged:
-  !cid T1 T2 M1 M2.
-    parstep cid T1 M1 T2 M2 ==>
-    !p s p' s'.
-      FLOOKUP T1 cid = SOME (Core cid p s)
-      /\ FLOOKUP T2 cid = SOME (Core cid p' s')
-      ==> p = p'
-Proof
-  rpt strip_tac
-  >> fs[parstep_cases]
-  >> last_assum (fn th => fs [th,FLOOKUP_UPDATE])
-QED
-
-Triviality latest_bound:
-!l t M.
-  latest l t M <= t
-Proof
-  Induct_on ‘t’ >> fs[latest_def]
-  >> rpt strip_tac
-  >> ‘latest l t M <= t’ by fs[]
-  >> Cases_on ‘oEL t M’
-  >> Cases_on ‘l = x.loc’
-  >> fs[]
-QED
-
-Triviality latest_exact:
-!l t M msg.
-  mem_get M l t = SOME msg
-  ==>
-  latest l t M = t
-Proof
-  Cases_on ‘t’
-  >> rpt strip_tac
-  >> fs[latest_def]
-  >> Cases_on ‘oEL n M’
-  >- fs[mem_get_def]
-  >> ‘x = msg’ by fs[mem_get_def]
-  >> ‘l = msg.loc’ by (drule mem_get_SOME >> fs[])
-  >> gvs[]
-QED
-
-Triviality latest_sound:
-  !l t M. ?msg.
-            mem_get M l (latest l t M) = SOME msg
-            /\ msg.loc = l
-Proof
-  Induct_on ‘t’ >- fs[latest_def, mem_get_def, mem_default_def]
-  >> rpt strip_tac
-  >> fs[latest_def]
-  >> Cases_on ‘oEL t M’
-  >> fs[]
-  >> Cases_on ‘l = x.loc’ >- fs[mem_get_def]
-  >> fs[]
-QED
-
-Theorem latest_is_latest:
-  !l t M t' msg.
-    latest l t M <= t' /\ t' <= t
-    /\ mem_get M l t' = SOME msg
-    ==>
-    t' = latest l t M
-Proof
-  Induct_on ‘t’ >- fs[latest_def]
-  >> rpt strip_tac
-  >> qspecl_then [‘l’, ‘SUC t’, ‘M’] assume_tac latest_sound
-  >> Cases_on ‘t' = SUC t’ >- fs[latest_exact]
-  >> ‘t' <= t’ by decide_tac
-  >> fs[latest_def]
-  >> Cases_on ‘oEL t M’
-  >> Cases_on ‘l = x.loc’
-  >> fs[]
-QED
-
-Theorem latest_monotonicity:
-!l M t1 t2.
-  t1 <= t2 ==> latest l t1 M <= latest l t2 M
-Proof
-  rpt strip_tac
-  >> ‘?msg.mem_get M l (latest l t2 M) = SOME msg /\ msg.loc = l’
-    by fs[latest_sound]
-  >> ‘latest l t1 M <= t1’ by fs[latest_bound]
-  >> ‘latest l t2 M <= t2’ by fs[latest_bound]
-  >> Cases_on ‘t1 <= latest l t2 M’
-  >| [fs[]
-      ,
-      ‘latest l t2 M < t1’ by decide_tac
-      >> ‘?msg.mem_get M l (latest l t1 M) = SOME msg /\ msg.loc = l’
-        by fs[latest_sound]
-      >> spose_not_then assume_tac
-      >> ‘latest l t2 M <= latest l t1 M’ by decide_tac
-      >> ‘latest l t1 M <= t2’ by decide_tac
-      >> ‘latest l t1 M = latest l t2 M’
-         by (irule latest_is_latest >> fs[])
-      >> fs[]]
-QED
-
-Theorem latest_spec:
-  !l t M l1.
-    (l1 = latest l t M)
-    ==>
-    (?msg.
-      mem_get M l l1 = SOME msg
-      /\ msg.loc = l
-      /\
-      !t'. l1 < t' /\ t' <= t
-           ==>
-           mem_get M l t' = NONE)
-Proof
-  rpt strip_tac
-  >> qspecl_then [‘l’, ‘t’, ‘M’] assume_tac latest_sound
-  >> fs[]
-  >> rpt strip_tac
-  >> spose_not_then assume_tac
-  >> Cases_on ‘mem_get M l t'’ >- fs[]
-  >> ‘latest l t' M = t'’ by fs[latest_exact]
-  >> ‘latest l t' M <= latest l t M’ by fs[latest_monotonicity]
-  >> rw[]
-QED
-
-Theorem latest_idempotency:
-  !l t M.
-    latest l (latest l t M) M = latest l t M
-Proof
-  rpt strip_tac
-  >> ‘?msg. mem_get M l (latest l t M) = SOME msg /\ msg.loc = l’
-    by fs[latest_sound]
-  >> fs[latest_exact]
-QED
-
-Theorem latest_max:
-!l M t1 t2.
-   latest l t1 M <= latest l (MAX t1 t2) M
-   /\ latest l t2 M <= latest l (MAX t1 t2) M
-Proof
-  fs[latest_monotonicity]
-QED
-
-Theorem clstep_preserves_wf_fwdb:
-!p cid s M prom s'.
-(!l. well_formed_fwdb l M (s.bst_coh l) (s.bst_fwdb l))
-/\ clstep p cid s M prom s'
-==>
-(!l. well_formed_fwdb l M (s'.bst_coh l) (s'.bst_fwdb l))
-Proof
-rpt strip_tac
->> fs[clstep_cases]
->> fs[well_formed_fwdb_def, latest_def]
->|
-[ (* read *)
-Cases_on ‘l = l'’
->| [
-‘(s.bst_fwdb l').fwdb_time ≤ latest l' (s.bst_coh l') M’ by fs[]
->> suff_tac “latest l' (s.bst_coh l') M <=
-             latest l'
-                    (MAX (s.bst_coh l')
-                     (MAX
-                      (MAX
-                       (MAX (MAX v_addr s.bst_v_rNew)
-                        (if acq ∧ rel then s.bst_v_Rel else 0))
-                       (if acq ∧ rel then MAX s.bst_v_rOld s.bst_v_wOld else 0))
-                      (mem_read_view (s.bst_fwdb l') t))) M” >- fs[]
->> fs[latest_max]
-,
-fs[]
-],
-  (* write *)
-  Cases_on ‘l = l'’
-  >| [
-    ‘mem_read M l' v_post = SOME v’ by fs[mem_read_def]
-    >> fs[]
-    >> ‘v_post = latest l' v_post M’ by fs[latest_exact]
-    >> ‘latest l' v_post M <= latest l' (MAX (s.bst_coh l') v_post) M’ suffices_by fs[]
-    >> fs[latest_max]
-    , fs[]
-  ]
-  , (* amo *)
-  Cases_on ‘l = l'’
-  >| [
-      EVAL_TAC
-      >> ‘mem_read M l t_w = SOME v_w’ by fs[mem_read_def]
-      >> fs[]
-      >> ‘t_w = latest l t_w M’  by fs[latest_exact]
-      >> ‘latest l' t_w M <= latest l' (MAX (s.bst_coh l') t_w) M’
-         suffices_by gvs[]
-      >> fs[latest_max]
-      ,
-      EVAL_TAC
-      >> fs[]
-      >> ‘?v.mem_read M l (s.bst_fwdb l).fwdb_time = SOME v’ by fs[]
-      >> qexists_tac ‘v’
-      >> ‘?m. mem_get M l (s.bst_fwdb l).fwdb_time = SOME m /\ m.val = v’ by fs[mem_get_mem_read]
-      >> fs[]
-    ]
-  ,
-  (* branch *)
-  drule bir_exec_stmt_mc_invar >> strip_tac >> fs[]
-  ,
-  (* generic *)
-  drule bir_exec_stmt_mc_invar >> strip_tac >> fs[]
-]
-QED
-
-Theorem bir_eval_view_of_exp_wf:
-!a_e env viewenv M v_addr.
- well_formed_viewenv viewenv M
- /\ v_addr = bir_eval_view_of_exp a_e viewenv
- ==>
- v_addr <= LENGTH M
-Proof
-  fs[well_formed_viewenv_def]
-  >> Induct_on ‘a_e’
-  >> fs[bir_eval_view_of_exp_def]
-  >> rpt strip_tac
-  >- (Cases_on ‘FLOOKUP viewenv b’ >- fs[]
-      >> first_assum drule >> fs[])
-  >> first_assum drule
-  >> last_assum drule >> fs[]
-QED
-
-Triviality mem_read_view_wf_fwdb:
-!l M coh_t fwd t.
-well_formed_fwdb l M coh_t fwd
-/\ t <= LENGTH M
-==>
-mem_read_view fwd t ≤ LENGTH M
-Proof
-  rpt strip_tac
-  >> fs[mem_read_view_def, well_formed_fwdb_def]
-  >> CASE_TAC
-  >> gvs[]
-QED
-
-Theorem clstep_preserves_wf:
-!p cid s M prom s'.
-  well_formed cid M s
-  /\ clstep p cid s M prom s'
-==>
-  well_formed cid M s'
-Proof
-  cheat
-QED
-(* Incomplete proof for time reasons,
-   but it should be straightforward
-
-  rpt strip_tac
-  >> fs[well_formed_def]
-  >> drule_then imp_res_tac clstep_preserves_wf_fwdb
-  >> fs[clstep_cases]
-    >|
-  [ (* read *)
-    ‘v_addr <= LENGTH M’
-     by (fs[bir_eval_exp_view_def]
-         >> drule bir_eval_view_of_exp_wf
-         >> fs[])
-    >> fs[well_formed_viewenv_def]
-    >> Cases_on ‘acq /\ rel’
-    >|
-    [
-      irule_at Any mem_read_view_wf_fwdb
-      >> qexists_tac ‘l’ >> qexists_tac ‘s.bst_coh l’
-      >> gvs[]
-      >> conj_asm1_tac
-      >-
-        (‘t <= LENGTH M \/ (t = 0 /\ v = mem_default_value)’
-         by metis_tac[mem_read_some]
-         >> fs[])
-      >> rw[]
-      >> Cases_on ‘var' = var’
-      >> gvs[FLOOKUP_DEF, FLOOKUP_UPDATE]
-      >> irule mem_read_view_wf_fwdb
-      >> fs[]
-      >> qexists_tac ‘s.bst_coh l’ >> qexists_tac ‘l’
-      >> fs[]
-      ,
-      cheat
-    ]
-  , proof follows here
-  ]
-*)
-
-Definition valid_index_def:
-valid_index i rho =
-(i >= 0 /\ i < LENGTH rho)
-End
-
-Definition low_eq_view_def:
-low_eq_view (N:num) v1 v2 =
-  if v1 <= N /\ v2 <= N then v1 = v2 else T
-End
-
-Definition low_eq_fwd_def:
-low_eq_fwd (N:num) fwd1 fwd2 =
-  low_eq_view N fwd1.fwdb_view fwd2.fwdb_view
-End
-
-Definition low_eq_xclb_def:
-low_eq_xclb N (SOME xcl1) (SOME xcl2) =
-  low_eq_view N xcl1.xclb_view xcl2.xclb_view
-/\ low_eq_xclb N _ _ = T
-End
-
-Definition low_eq_def:
-low_eq (N:num) s s' =
-(low_eq_view N s.bst_v_rOld s'.bst_v_rOld
- /\ low_eq_view N s.bst_v_wOld s'.bst_v_wOld
- /\ low_eq_view N s.bst_v_rNew s'.bst_v_rNew
- /\ low_eq_view N s.bst_v_wNew s'.bst_v_wNew
- /\ low_eq_view N s.bst_v_CAP s'.bst_v_CAP
- /\ low_eq_view N s.bst_v_Rel s'.bst_v_Rel
- /\ (!var v1 v2.
-       FLOOKUP s.bst_viewenv var = SOME v1
-       /\ FLOOKUP s'.bst_viewenv var = SOME v2
-       ==> low_eq_view N v1 v2)
- /\ (!l. low_eq_view N (s.bst_coh l) (s'.bst_coh l))
- /\ (!l. low_eq_fwd N (s.bst_fwdb l) (s'.bst_fwdb l))
- /\ low_eq_xclb N s.bst_xclb s'.bst_xclb
-)
-End
-
-(* Monotonicity of vCAP *)
-
-(* Monotonicity of fence? *)
-
-(*Unwinding conditions
-
-NI-like lemma:
-cstep_seq_time p cid t s M s1 M'
-/\ low_eq k s s'
-==>
-?s2 t'.
-cstep_seq_time p cid t' s' M s2 M'
-/\ low-eq k s1 s2
-*)
-
-Definition is_read_stmt_def:
-  is_read_stmt p s l t v_pre =
-  ?M var a_e opt_cast xcl acq rel v_addr v.
-    bir_get_stmt p s.bst_pc =
-    BirStmt_Read var a_e opt_cast xcl acq rel
-    /\ (SOME l, v_addr) = bir_eval_exp_view a_e s.bst_environ s.bst_viewenv
-    /\ mem_read M l t = SOME v
-    /\ v_pre = MAX (MAX (MAX v_addr s.bst_v_rNew) (if (acq /\ rel) then s.bst_v_Rel else 0))
-                   (if (acq /\ rel) then (MAX s.bst_v_rOld s.bst_v_wOld) else 0)
-End
-
-(* Some attempts at formulating
-   the NI-like properties:
-
-Theorem unwinding_cstep_seq:
-!p cid t s M s1 M' k.
-  cstep_seq_time p cid t s M s1 M'
-  /\ low_eq k s s'
-  ==>
-  ?s2 t'.
-    (cstep_seq_time p cid t' s' M s2 M'
-     /\ low-eq k s1 s2)
-Proof
-  cheat
-QED
-
-Theorem cert_future_irrelevance:
-!p cid s M rho i j.
-rho IN certifying_traces p cid s M
-valid_index i rho /\ valid_index j rho
-/\ time = timestamp_at i rho
-/\ is_mem_op i rho
-/\ timestamp_at j rho > time
-==>
-!rho'.
-similar_trace rho rho' (* ?? *)
-/\ ~(timestamp_at j rho' = timestamp_at j rho)
-/\ timestamp_at j rho' = LENGTH M + 1 (* ?? *)
-==>
-rho' IN certifying_traces p cid s (M++[promise]) (* ?? *)
-Proof
-  cheat
-QED
-*)
-
-Triviality mem_read_append:
-!t M l msg.
-     t <= LENGTH M ==> mem_read (M++[msg]) l t = mem_read M l t
-Proof
-  fs[mem_read_def,mem_get_append]
-QED
-
-(* More general version, but not needed so far
-Triviality mem_read_append2:
-  !t M l M'.
-    t <= LENGTH M ==> mem_read (M++M') l t = mem_read M l t
-Proof
-  rewrite_tac [GSYM listTheory.SNOC_APPEND]
-  >> Induct_on ‘t’
-  >> fs[mem_read_def]
-  >> rpt strip_tac
-  >> rw[mem_read_def, mem_get_def]
-  >> fs[listTheory.oEL_THM, listTheory.EL_SNOC, listTheory.EL_APPEND_EQN]
-QED
-*)
 
 Theorem promise_inversion:
 !cid cores M cores' M'.
@@ -731,7 +230,8 @@ QED
 
 Theorem promises_do_not_disable_clsteps:
 ! msg p s s' M1 prom.
-clstep p msg.cid s M1 prom s'
+well_formed msg.cid M1 s
+/\ clstep p msg.cid s M1 prom s'
 ==>
 clstep p msg.cid
       (s with bst_prom updated_by (λpr. pr ⧺ [LENGTH M1 + 1]))
@@ -749,11 +249,17 @@ Induct_on ‘clstep’
   [drule mem_read_some >> strip_tac >> fs[mem_read_append]
   ,fs[]
   , (* quantifier case *)
-  qpat_assum ‘!t''._’ (fn th => drule (Q.SPEC ‘t'’ th))
+  ‘t' <= LENGTH M1’ by (* wf invariant *)
+    (‘v_addr <= LENGTH M1’ by metis_tac[well_formed_def, bir_eval_exp_view_bound]
+     >> ‘v_pre <= LENGTH M1’ by
+       (Cases_on ‘acq /\ rel’ >> fs[well_formed_def])
+     >> ‘MAX v_pre
+         ((s with bst_prom updated_by (λpr. pr ⧺ [LENGTH M1 + 1])).bst_coh l) <= LENGTH M1’ by fs[well_formed_def, bir_programTheory.bir_state_t_accfupds]
+     >> decide_tac)
+  >> qpat_assum ‘!t''._’ (fn th => drule (Q.SPEC ‘t'’ th))
   >> rpt strip_tac
   >> ‘¬mem_is_loc M1 t' l’ by fs[]
   >> fs[listTheory.oEL_EQ_EL, listTheory.EL_APPEND_EQN]
-  >> ‘t' <= LENGTH M1’ by cheat (* wf invariant should cover this *)
   >> fs[GSYM mem_get_is_loc, optionTheory.IS_SOME_EXISTS]
   >> fs[mem_get_append]
   ,fs[]
@@ -769,7 +275,7 @@ Induct_on ‘clstep’
   >> fs[bir_programTheory.bir_state_t_accfupds]
   >> Q.LIST_EXISTS_TAC [‘v’,‘l’,‘v_addr’,‘v_data’,‘new_env’, ‘new_viewenv’]
   >> gvs[fulfil_atomic_ok_def, fulfil_update_env_def, fulfil_update_viewenv_def, listTheory.oEL_EQ_EL, listTheory.EL_APPEND_EQN]
-  >> ‘t <= LENGTH M1’ by cheat (* wf invariant *)
+  >> ‘t <= LENGTH M1’ by fs[well_formed_def] (* wf invariant *)
   >> rpt strip_tac
   >| [
       fs[mem_is_cid_def] >> cheat (* proof obligation about mem_is_cide *)
@@ -790,7 +296,7 @@ Induct_on ‘clstep’
   >> fs[bir_programTheory.bir_state_t_accfupds]
   >> Q.LIST_EXISTS_TAC [‘v_addr’, ‘v_data’, ‘l’, ‘v_r’, ‘v_w’, ‘t_r’, ‘new_environ’]
   >> gvs[fulfil_atomic_ok_def, fulfil_update_env_def, fulfil_update_viewenv_def, listTheory.oEL_EQ_EL, listTheory.EL_APPEND_EQN]
-  >> ‘t_w <= LENGTH M1’ by cheat (* wf invariant *)
+  >> ‘t_w <= LENGTH M1’ by fs[well_formed_def] (* wf invariant *)
   >> rpt strip_tac
   >| [drule mem_read_some >> strip_tac >> fs[mem_read_append]
       ,
@@ -837,6 +343,8 @@ Induct_on ‘clstep’
 ]
 QED
 
+
+
 Theorem certification_extension:
 !p cid M s s'' msg prom.
   is_certified p cid s'' M
@@ -845,6 +353,7 @@ Theorem certification_extension:
       (M ⧺ [msg])
   /\ msg.cid = cid
   /\ cstep p cid s M prom s'' M
+  /\ well_formed cid M s
 ==>
   is_certified p cid
     (s with bst_prom updated_by (λpr. pr ⧺ [LENGTH M + 1]))
@@ -867,6 +376,7 @@ Theorem nonpromising_extra_promise:
   parstep msg.cid (T1 |+ (msg.cid,Core msg.cid p s')) M1
               (T1 |+ (msg.cid,Core msg.cid p s)) M1
   /\ is_certified p msg.cid (s with bst_prom updated_by (\pr. pr ++ [LENGTH M1 + 1])) (M1 ++ [msg])
+  /\ well_formed msg.cid M1 s'
   ==>
   parstep msg.cid (T1 |+ (msg.cid,Core msg.cid p (s' with bst_prom updated_by (\pr. pr ++ [LENGTH M1 + 1])))) (M1 ++ [msg])
           (T1 |+ (msg.cid,Core msg.cid p (s with bst_prom updated_by (\pr. pr ++ [LENGTH M1 + 1])))) (M1 ++ [msg])
@@ -877,7 +387,8 @@ Proof
   >> Q.EXISTS_TAC ‘prom’
   >> fs[FLOOKUP_UPDATE]
   >> fs[atomicity_ok_def]
-  >> fs[cstep_cases, promises_do_not_disable_clsteps]
+  >> fs[cstep_cases]
+  >> gvs[promises_do_not_disable_clsteps]
 QED
 
 Theorem bir_promising_diamond_same_core:
@@ -898,27 +409,25 @@ Proof
 >> fs[FLOOKUP_UPDATE] (* introduces p = p' and s = s'' *)
 >> Q.EXISTS_TAC ‘FUPDATE T1 (msg.cid, Core msg.cid p (s with bst_prom updated_by (λpr. pr ⧺ [LENGTH M1 + 1])))’
 >> Q.PAT_ASSUM ‘p=p'’ (fn th => once_rewrite_tac [th])
->> ‘is_certified p' msg.cid (s with bst_prom updated_by (\pr. pr ++ [LENGTH M1 + 1])) (M1 ++ [msg])’ by (
+>> ‘is_certified p' msg.cid (s with bst_prom updated_by (\pr. pr ++ [LENGTH M1 + 1])) (M1 ++ [msg])’ by (cheat
+  (*
   match_mp_tac certification_extension
   >> Q.LIST_EXISTS_TAC [‘s''’, ‘prom’]
-  >> fs[]
+  >> fs[] *)
    )
 >> ‘cstep p' msg.cid s M1 [LENGTH M1 + 1] (s with bst_prom updated_by (\pr. pr ++ [LENGTH M1 + 1])) (M1 ++ [msg])’ by rw[cstep_rules]
 >> strip_tac >| [
     match_mp_tac parstep_rules >> Q.EXISTS_TAC ‘s’ >> Q.EXISTS_TAC ‘[LENGTH M1 + 1]’ >> fs[],
-    ‘parstep msg.cid (T1 |+ (msg.cid, Core msg.cid p' s))
-     M1
-     (T1 |+ (msg.cid, Core msg.cid p' s''))
-     M1’ by (
-      ‘T1 |+ (msg.cid, Core msg.cid p' s) = T1’ by fs[flookup_thm,FUPDATE_ELIM] >> fs[])
-    >> dxrule nonpromising_extra_promise
-    >> fs[FUPDATE_EQ]
+    irule nonpromising_extra_promise
+    >> fs[flookup_thm,FUPDATE_ELIM]
+    >> cheat
     ]
 QED
 
 Theorem promises_do_not_disable_clsteps_other_core:
 !p cid M prom s s' msg.
 ~(cid = msg.cid)
+/\ well_formed cid M s
 /\ clstep p cid s M prom s'
 ==>
 clstep p cid s (M++[msg]) prom s'
@@ -933,7 +442,13 @@ Proof
     [drule mem_read_some >> strip_tac >> fs[mem_read_append]
      ,fs[]
      , (* quantifier case *)
-     ‘t' <= LENGTH M’ by cheat (* wf invariant *)
+     (* using the wf invariant *)
+     ‘t' <= LENGTH M’ by
+       (‘v_addr <= LENGTH M’ by metis_tac[well_formed_def, bir_eval_exp_view_bound]
+        >> ‘v_pre <= LENGTH M’ by
+          (Cases_on ‘acq /\ rel’ >> fs[well_formed_def])
+        >> ‘MAX v_pre (s.bst_coh l) <= LENGTH M’ by fs[well_formed_def]
+        >> decide_tac)
      >> qpat_assum ‘!t''._’ (fn th => drule (Q.SPEC ‘t'’ th))
      >> rpt strip_tac
      >> ‘t' ≤ MAX v_pre (s.bst_coh l)’ by fs[bir_state_t_accfupds]
@@ -955,13 +470,13 @@ Proof
     >> Q.LIST_EXISTS_TAC [‘v’,‘l’,‘v_addr’,‘v_data’,‘new_env’, ‘new_viewenv’]
     >> gvs[fulfil_atomic_ok_def, fulfil_update_env_def, fulfil_update_viewenv_def, listTheory.oEL_EQ_EL, listTheory.EL_APPEND_EQN]
     >> rpt strip_tac >- cheat (* mem_is_cid *)
-    >> ‘t <= LENGTH M’ by cheat (* wf invariant *)
+    >> ‘t <= LENGTH M’ by fs[well_formed_def] (* wf invariant *)
     >> fs[mem_get_append]
     ,(* amo *)
     HO_MATCH_MP_TAC (List.nth (CONJUNCTS clstep_rules,3))
     >> fs[bir_programTheory.bir_state_t_accfupds]
     >> Q.LIST_EXISTS_TAC [‘v_addr’, ‘v_data’, ‘l’, ‘v_r’, ‘v_w’, ‘t_r’, ‘new_environ’]
-    >> ‘t_w <= LENGTH M’ by cheat (* wf invariant *)
+    >> ‘t_w <= LENGTH M’ by fs[well_formed_def] (* wf invariant *)
     >> gvs[fulfil_atomic_ok_def, fulfil_update_env_def, fulfil_update_viewenv_def, listTheory.oEL_EQ_EL, listTheory.EL_APPEND_EQN]
     >> rpt strip_tac
     >| [
@@ -995,6 +510,186 @@ Proof
   >> rpt HINT_EXISTS_TAC >> fs[]
   ]
 QED
+
+(* The following lemma is needed in the
+bir_promising_diamond_diff_core proof *)
+Theorem certification_extension_other_core:
+  !p p' cid s s' s'' M prom msg.
+    ~(cid = msg.cid)
+    /\ is_certified p cid s' M
+    /\ cstep p cid s M prom s' M
+    /\ is_certified (p':string bir_program_t) msg.cid s'' (M++[msg])
+    ==>
+    is_certified p cid s' (M++[msg])
+Proof
+ cheat
+QED
+
+Theorem bir_promising_diamond_diff_core:
+  !T1 T2 T3 M1 M2 M3 cid1 cid2.
+    (~(cid1 = cid2)
+    /\ nonpromise_step cid1 (T1,M1) (T2,M2)
+    /\ promise_step cid2 (T2,M2) (T3,M3))
+    ==>
+    ?T1' T2' T3' M1' M2' M3'.
+      (T1,M1) = (T1',M1')
+      /\ promise_step cid2 (T1',M1') (T2',M2')
+      /\ nonpromise_step cid1 (T2',M2') (T3',M3')
+      /\ (T3,M3) = (T3',M3')
+Proof
+  fs[bir_nonpromise_step_def, bir_promise_step_def]
+  >> rpt strip_tac
+  >> drule execute_inversion >> rw[]
+  >> drule promise_inversion  >> rw[]
+  >> fs[FLOOKUP_UPDATE]
+  >> Q.EXISTS_TAC ‘FUPDATE T1 (msg.cid, Core msg.cid p' (s'' with bst_prom updated_by (λpr. pr ⧺ [LENGTH M1 + 1])))’
+  >> strip_tac
+  >| [
+    match_mp_tac parstep_rules
+    >> Q.LIST_EXISTS_TAC [‘s''’, ‘[LENGTH M1+1]’]
+    >> fs[atomicity_ok_def, cstep_rules]
+    >> LAST_ASSUM (fn th => fs[th])
+    >> ‘cores_pc_not_atomic (T1 \\ msg.cid)’ by cheat
+    ,
+    FULL_SIMP_TAC std_ss [Once FUPDATE_COMMUTES]
+    >> match_mp_tac parstep_rules
+    >> Q.LIST_EXISTS_TAC [‘s’,‘prom’]
+    >> fs[FLOOKUP_UPDATE, atomicity_ok_def]
+    >> ‘cores_pc_not_atomic
+                (T1 |+
+                 (msg.cid,
+                  Core msg.cid p'
+                       (s'' with bst_prom updated_by (λpr. pr ⧺ [LENGTH M1 + 1]))) \\
+                 cid1)’ by cheat
+    >> rpt strip_tac >- fs[]
+    >| [ ‘well_formed cid1 M1 s’ by cheat (* this should follow from an assumption *)
+        >> fs[cstep_cases, promises_do_not_disable_clsteps_other_core]
+        ,HO_MATCH_MP_TAC certification_extension_other_core
+         >> Q.LIST_EXISTS_TAC
+             [‘p'’, ‘s’,
+              ‘(s'' with bst_prom updated_by (\pr. pr ++ [LENGTH M1 + 1]))’
+              ,‘prom’]
+      >> fs[]
+      ]
+]
+QED
+  
+(*
+=============================================
+Experimental/unfinished stuff after this line
+*)
+Definition valid_index_def:
+valid_index i rho =
+(i >= 0 /\ i < LENGTH rho)
+End
+
+Definition low_eq_view_def:
+low_eq_view (N:num) v1 v2 =
+  if v1 <= N /\ v2 <= N then v1 = v2 else T
+End
+
+Definition low_eq_fwd_def:
+low_eq_fwd (N:num) fwd1 fwd2 =
+  low_eq_view N fwd1.fwdb_view fwd2.fwdb_view
+End
+
+Definition low_eq_xclb_def:
+low_eq_xclb N (SOME xcl1) (SOME xcl2) =
+  low_eq_view N xcl1.xclb_view xcl2.xclb_view
+/\ low_eq_xclb N _ _ = T
+End
+
+Definition low_eq_def:
+low_eq (N:num) s s' =
+(low_eq_view N s.bst_v_rOld s'.bst_v_rOld
+ /\ low_eq_view N s.bst_v_wOld s'.bst_v_wOld
+ /\ low_eq_view N s.bst_v_rNew s'.bst_v_rNew
+ /\ low_eq_view N s.bst_v_wNew s'.bst_v_wNew
+ /\ low_eq_view N s.bst_v_CAP s'.bst_v_CAP
+ /\ low_eq_view N s.bst_v_Rel s'.bst_v_Rel
+ /\ (!var v1 v2.
+       FLOOKUP s.bst_viewenv var = SOME v1
+       /\ FLOOKUP s'.bst_viewenv var = SOME v2
+       ==> low_eq_view N v1 v2)
+ /\ (!l. low_eq_view N (s.bst_coh l) (s'.bst_coh l))
+ /\ (!l. low_eq_fwd N (s.bst_fwdb l) (s'.bst_fwdb l))
+ /\ low_eq_xclb N s.bst_xclb s'.bst_xclb
+)
+End
+
+(* Monotonicity of vCAP *)
+
+(* Monotonicity of fence? *)
+
+(*Unwinding conditions
+
+NI-like lemma:
+cstep_seq_time p cid t s M s1 M'
+/\ low_eq k s s'
+==>
+?s2 t'.
+cstep_seq_time p cid t' s' M s2 M'
+/\ low-eq k s1 s2
+*)
+
+Definition is_read_stmt_def:
+  is_read_stmt p s l t v_pre =
+  ?M var a_e opt_cast xcl acq rel v_addr v.
+    bir_get_stmt p s.bst_pc =
+    BirStmt_Read var a_e opt_cast xcl acq rel
+    /\ (SOME l, v_addr) = bir_eval_exp_view a_e s.bst_environ s.bst_viewenv
+    /\ mem_read M l t = SOME v
+    /\ v_pre = MAX (MAX (MAX v_addr s.bst_v_rNew) (if (acq /\ rel) then s.bst_v_Rel else 0))
+                   (if (acq /\ rel) then (MAX s.bst_v_rOld s.bst_v_wOld) else 0)
+End
+
+(* Some attempts at formulating
+   the NI-like properties:
+
+Theorem unwinding_cstep_seq:
+!p cid t s M s1 M' k.
+  cstep_seq_time p cid t s M s1 M'
+  /\ low_eq k s s'
+  ==>
+  ?s2 t'.
+    (cstep_seq_time p cid t' s' M s2 M'
+     /\ low-eq k s1 s2)
+Proof
+  cheat
+QED
+
+Theorem cert_future_irrelevance:
+!p cid s M rho i j.
+rho IN certifying_traces p cid s M
+valid_index i rho /\ valid_index j rho
+/\ time = timestamp_at i rho
+/\ is_mem_op i rho
+/\ timestamp_at j rho > time
+==>
+!rho'.
+similar_trace rho rho' (* ?? *)
+/\ ~(timestamp_at j rho' = timestamp_at j rho)
+/\ timestamp_at j rho' = LENGTH M + 1 (* ?? *)
+==>
+rho' IN certifying_traces p cid s (M++[promise]) (* ?? *)
+Proof
+  cheat
+QED
+*)
+
+(* More general version, but not needed so far
+Triviality mem_read_append2:
+  !t M l M'.
+    t <= LENGTH M ==> mem_read (M++M') l t = mem_read M l t
+Proof
+  rewrite_tac [GSYM listTheory.SNOC_APPEND]
+  >> Induct_on ‘t’
+  >> fs[mem_read_def]
+  >> rpt strip_tac
+  >> rw[mem_read_def, mem_get_def]
+  >> fs[listTheory.oEL_THM, listTheory.EL_SNOC, listTheory.EL_APPEND_EQN]
+QED
+*)
 
 (* Latest version of the NI-like lemma
 if the step is a load
@@ -1057,6 +752,11 @@ Proof
   cheat]
 QED
 
+(* This one is missing the well-formedness assumption,
+   but it is probably not worth it to port since
+   it's not clear if this theorem will be needed in the
+   new approach
+
 Theorem promise_list_does_not_disable_cstep_seq:
   !cid p s M s' M'.
     (cstep_seq p cid (s,M) (s',M++M')
@@ -1090,6 +790,7 @@ Proof
       >> irule clstep_fulfil_other_core >> gvs[]
      ]
 QED
+*)
 
 (* Some minor lemmas about cstep_seq *)
 
@@ -1143,66 +844,17 @@ Proof
 QED
 *)
 
-(* The following lemma is needed in the
-bir_promising_diamond_diff_core proof *)
-Theorem certification_extension_other_core:
-  !p p' cid s s' s'' M prom msg.
-    ~(cid = msg.cid)
-    /\ is_certified p cid s' M
-    /\ cstep p cid s M prom s' M
-    /\ is_certified (p':string bir_program_t) msg.cid s'' (M++[msg])
-    ==>
-    is_certified p cid s' (M++[msg])
+Theorem programs_unchanged:
+  !cid T1 T2 M1 M2.
+    parstep cid T1 M1 T2 M2 ==>
+    !p s p' s'.
+      FLOOKUP T1 cid = SOME (Core cid p s)
+      /\ FLOOKUP T2 cid = SOME (Core cid p' s')
+      ==> p = p'
 Proof
- cheat
+  rpt strip_tac
+  >> fs[parstep_cases]
+  >> last_assum (fn th => fs [th,FLOOKUP_UPDATE])
 QED
-
-Theorem bir_promising_diamond_diff_core:
-  !T1 T2 T3 M1 M2 M3 cid1 cid2.
-    (~(cid1 = cid2)
-    /\ nonpromise_step cid1 (T1,M1) (T2,M2)
-    /\ promise_step cid2 (T2,M2) (T3,M3))
-    ==>
-    ?T1' T2' T3' M1' M2' M3'.
-      (T1,M1) = (T1',M1')
-      /\ promise_step cid2 (T1',M1') (T2',M2')
-      /\ nonpromise_step cid1 (T2',M2') (T3',M3')
-      /\ (T3,M3) = (T3',M3')
-Proof
-  fs[bir_nonpromise_step_def, bir_promise_step_def]
-  >> rpt strip_tac
-  >> drule execute_inversion >> rw[]
-  >> drule promise_inversion  >> rw[]
-  >> fs[FLOOKUP_UPDATE]
-  >> Q.EXISTS_TAC ‘FUPDATE T1 (msg.cid, Core msg.cid p' (s'' with bst_prom updated_by (λpr. pr ⧺ [LENGTH M1 + 1])))’
-  >> strip_tac
-  >| [
-    match_mp_tac parstep_rules
-    >> Q.LIST_EXISTS_TAC [‘s''’, ‘[LENGTH M1+1]’]
-    >> fs[atomicity_ok_def, cstep_rules]
-    >> LAST_ASSUM (fn th => fs[th])
-    >> ‘cores_pc_not_atomic (T1 \\ msg.cid)’ by cheat
-    ,
-    FULL_SIMP_TAC std_ss [Once FUPDATE_COMMUTES]
-    >> match_mp_tac parstep_rules
-    >> Q.LIST_EXISTS_TAC [‘s’,‘prom’]
-    >> fs[FLOOKUP_UPDATE, atomicity_ok_def]
-    >> ‘cores_pc_not_atomic
-                (T1 |+
-                 (msg.cid,
-                  Core msg.cid p'
-                       (s'' with bst_prom updated_by (λpr. pr ⧺ [LENGTH M1 + 1]))) \\
-                 cid1)’ by cheat
-    >> rpt strip_tac >- fs[]
-    >| [fs[cstep_cases, promises_do_not_disable_clsteps_other_core]
-        ,HO_MATCH_MP_TAC certification_extension_other_core
-         >> Q.LIST_EXISTS_TAC
-             [‘p'’, ‘s’,
-              ‘(s'' with bst_prom updated_by (\pr. pr ++ [LENGTH M1 + 1]))’
-              ,‘prom’]
-      >> fs[]
-      ]
-]
-QED
-
+  
 val _ = export_theory ()
