src/theory/bir/bir_promising_wfScript.sml
@@ -1,0 +1,351 @@
+open HolKernel Parse boolLib bossLib;
+open bir_promisingTheory;
+open bir_programTheory;
+open bir_valuesTheory;
+open bir_expTheory;
+open finite_mapTheory;
+
+val _ = new_theory "bir_promising_wf";
+
+Definition latest_def:
+  latest l 0 M = 0
+  /\ latest l (SUC t) M =
+  case oEL t M of
+    SOME msg =>
+      if l = msg.loc then SUC t else latest l t M
+  | _ => latest l t M
+End
+
+Definition well_formed_fwdb_def:
+ well_formed_fwdb l M coh_t fwd =
+   (fwd.fwdb_time <= latest l coh_t M
+    /\ fwd.fwdb_view <= fwd.fwdb_time
+    /\ ?v. mem_read M l fwd.fwdb_time = SOME v)
+End
+(*
+Definition well_formed_xclb_def:
+  well_formed_xclb M coh_t xclb =
+  (xclb.xclb_time <= latest xclb.xclb_loc coh_t M
+   /\ xclb.xclb_view <= coh_t
+   /\ ?v. mem_read M xclb.xclb_loc xclb.xclb_time = SOME v)
+End
+*)
+
+Definition well_formed_viewenv_def:
+  well_formed_viewenv viewenv M =
+  !var v. FLOOKUP viewenv var = SOME v
+  ==>
+  v <= LENGTH M
+End
+
+Definition well_formed_def:
+  well_formed cid M s =
+  ( well_formed_viewenv s.bst_viewenv M
+    /\ (!l. s.bst_coh(l) <= LENGTH M)
+     /\ s.bst_v_rNew <= LENGTH M
+     /\ s.bst_v_rOld <= LENGTH M
+     /\ s.bst_v_wNew <= LENGTH M
+     /\ s.bst_v_wOld <= LENGTH M
+     /\ s.bst_v_CAP <= LENGTH M
+     /\ s.bst_v_Rel <= LENGTH M
+     /\ (!l. well_formed_fwdb l M (s.bst_coh(l)) (s.bst_fwdb(l)))
+(*     /\ (!xclb. s.bst_xclb = SOME xclb ==> well_formed_xclb M (s.bst_coh(xclb.loc) xclb)) *)
+     /\ (!t. MEM t s.bst_prom ==> t <= LENGTH M)
+     /\ (!t msg.
+           (oEL t M = SOME msg
+            /\ msg.cid = cid
+            /\ s.bst_coh(msg.loc) < t)
+           ==>
+           MEM t s.bst_prom)
+    )
+End
+    
+Theorem latest_bound:
+!l t M.
+  latest l t M <= t
+Proof
+  Induct_on ‘t’ >> fs[latest_def]
+  >> rpt strip_tac
+  >> ‘latest l t M <= t’ by fs[]
+  >> Cases_on ‘oEL t M’
+  >> Cases_on ‘l = x.loc’
+  >> fs[]
+QED
+
+Theorem latest_exact:
+!l t M msg.
+  mem_get M l t = SOME msg
+  ==>
+  latest l t M = t
+Proof
+  Cases_on ‘t’
+  >> rpt strip_tac
+  >> fs[latest_def]
+  >> Cases_on ‘oEL n M’
+  >- fs[mem_get_def]
+  >> ‘x = msg’ by fs[mem_get_def]
+  >> ‘l = msg.loc’ by (drule mem_get_SOME >> fs[])
+  >> gvs[]
+QED
+
+Theorem latest_sound:
+  !l t M. ?msg.
+            mem_get M l (latest l t M) = SOME msg
+            /\ msg.loc = l
+Proof
+  Induct_on ‘t’ >- fs[latest_def, mem_get_def, mem_default_def]
+  >> rpt strip_tac
+  >> fs[latest_def]
+  >> Cases_on ‘oEL t M’
+  >> fs[]
+  >> Cases_on ‘l = x.loc’ >- fs[mem_get_def]
+  >> fs[]
+QED
+
+Theorem latest_is_latest:
+  !l t M t' msg.
+    latest l t M <= t' /\ t' <= t
+    /\ mem_get M l t' = SOME msg
+    ==>
+    t' = latest l t M
+Proof
+  Induct_on ‘t’ >- fs[latest_def]
+  >> rpt strip_tac
+  >> qspecl_then [‘l’, ‘SUC t’, ‘M’] assume_tac latest_sound
+  >> Cases_on ‘t' = SUC t’ >- fs[latest_exact]
+  >> ‘t' <= t’ by decide_tac
+  >> fs[latest_def]
+  >> Cases_on ‘oEL t M’
+  >> Cases_on ‘l = x.loc’
+  >> fs[]
+QED
+
+Theorem latest_monotonicity:
+!l M t1 t2.
+  t1 <= t2 ==> latest l t1 M <= latest l t2 M
+Proof
+  rpt strip_tac
+  >> ‘?msg.mem_get M l (latest l t2 M) = SOME msg /\ msg.loc = l’
+    by fs[latest_sound]
+  >> ‘latest l t1 M <= t1’ by fs[latest_bound]
+  >> ‘latest l t2 M <= t2’ by fs[latest_bound]
+  >> Cases_on ‘t1 <= latest l t2 M’
+  >| [fs[]
+      ,
+      ‘latest l t2 M < t1’ by decide_tac
+      >> ‘?msg.mem_get M l (latest l t1 M) = SOME msg /\ msg.loc = l’
+        by fs[latest_sound]
+      >> spose_not_then assume_tac
+      >> ‘latest l t2 M <= latest l t1 M’ by decide_tac
+      >> ‘latest l t1 M <= t2’ by decide_tac
+      >> ‘latest l t1 M = latest l t2 M’
+         by (irule latest_is_latest >> fs[])
+      >> fs[]]
+QED
+
+Theorem latest_spec:
+  !l t M l1.
+    (l1 = latest l t M)
+    ==>
+    (?msg.
+      mem_get M l l1 = SOME msg
+      /\ msg.loc = l
+      /\
+      !t'. l1 < t' /\ t' <= t
+           ==>
+           mem_get M l t' = NONE)
+Proof
+  rpt strip_tac
+  >> qspecl_then [‘l’, ‘t’, ‘M’] assume_tac latest_sound
+  >> fs[]
+  >> rpt strip_tac
+  >> spose_not_then assume_tac
+  >> Cases_on ‘mem_get M l t'’ >- fs[]
+  >> ‘latest l t' M = t'’ by fs[latest_exact]
+  >> ‘latest l t' M <= latest l t M’ by fs[latest_monotonicity]
+  >> rw[]
+QED
+
+Theorem latest_idempotency:
+  !l t M.
+    latest l (latest l t M) M = latest l t M
+Proof
+  rpt strip_tac
+  >> ‘?msg. mem_get M l (latest l t M) = SOME msg /\ msg.loc = l’
+    by fs[latest_sound]
+  >> fs[latest_exact]
+QED
+
+Theorem latest_max:
+!l M t1 t2.
+   latest l t1 M <= latest l (MAX t1 t2) M
+   /\ latest l t2 M <= latest l (MAX t1 t2) M
+Proof
+  fs[latest_monotonicity]
+QED
+
+
+Theorem clstep_preserves_wf_fwdb:
+!p cid s M prom s'.
+(!l. well_formed_fwdb l M (s.bst_coh l) (s.bst_fwdb l))
+/\ clstep p cid s M prom s'
+==>
+(!l. well_formed_fwdb l M (s'.bst_coh l) (s'.bst_fwdb l))
+Proof
+rpt strip_tac
+>> fs[clstep_cases]
+>> fs[well_formed_fwdb_def, latest_def]
+>|
+[ (* read *)
+Cases_on ‘l = l'’
+>| [
+‘(s.bst_fwdb l').fwdb_time ≤ latest l' (s.bst_coh l') M’ by fs[]
+>> suff_tac “latest l' (s.bst_coh l') M <=
+             latest l'
+                    (MAX (s.bst_coh l')
+                     (MAX
+                      (MAX
+                       (MAX (MAX v_addr s.bst_v_rNew)
+                        (if acq ∧ rel then s.bst_v_Rel else 0))
+                       (if acq ∧ rel then MAX s.bst_v_rOld s.bst_v_wOld else 0))
+                      (mem_read_view (s.bst_fwdb l') t))) M” >- fs[]
+>> fs[latest_max]
+,
+fs[]
+],
+  (* write *)
+  Cases_on ‘l = l'’
+  >| [
+    ‘mem_read M l' v_post = SOME v’ by fs[mem_read_def]
+    >> fs[]
+    >> ‘v_post = latest l' v_post M’ by fs[latest_exact]
+    >> ‘latest l' v_post M <= latest l' (MAX (s.bst_coh l') v_post) M’ suffices_by fs[]
+    >> fs[latest_max]
+    , fs[]
+  ]
+  , (* amo *)
+  Cases_on ‘l = l'’
+  >| [
+      EVAL_TAC
+      >> ‘mem_read M l t_w = SOME v_w’ by fs[mem_read_def]
+      >> fs[]
+      >> ‘t_w = latest l t_w M’  by fs[latest_exact]
+      >> ‘latest l' t_w M <= latest l' (MAX (s.bst_coh l') t_w) M’
+         suffices_by gvs[]
+      >> fs[latest_max]
+      ,
+      EVAL_TAC
+      >> fs[]
+      >> ‘?v.mem_read M l (s.bst_fwdb l).fwdb_time = SOME v’ by fs[]
+      >> qexists_tac ‘v’
+      >> ‘?m. mem_get M l (s.bst_fwdb l).fwdb_time = SOME m /\ m.val = v’ by fs[mem_get_mem_read]
+      >> fs[]
+    ]
+  ,
+  (* branch *)
+  drule bir_exec_stmt_mc_invar >> strip_tac >> fs[]
+  ,
+  (* generic *)
+  drule bir_exec_stmt_mc_invar >> strip_tac >> fs[]
+]
+QED
+
+Theorem bir_eval_view_of_exp_wf:
+!a_e env viewenv M v_addr.
+ well_formed_viewenv viewenv M
+ /\ v_addr = bir_eval_view_of_exp a_e viewenv
+ ==>
+ v_addr <= LENGTH M
+Proof
+  fs[well_formed_viewenv_def]
+  >> Induct_on ‘a_e’
+  >> fs[bir_eval_view_of_exp_def]
+  >> rpt strip_tac
+  >- (Cases_on ‘FLOOKUP viewenv b’ >- fs[]
+      >> first_assum drule >> fs[])
+  >> first_assum drule
+  >> last_assum drule >> fs[]
+QED
+
+Theorem mem_read_view_wf_fwdb:
+!l M coh_t fwd t.
+well_formed_fwdb l M coh_t fwd
+/\ t <= LENGTH M
+==>
+mem_read_view fwd t ≤ LENGTH M
+Proof
+  rpt strip_tac
+  >> fs[mem_read_view_def, well_formed_fwdb_def]
+  >> CASE_TAC
+  >> gvs[]
+QED
+
+Theorem bir_eval_view_of_exp_bound:
+  !a_e s M.
+    well_formed_viewenv s.bst_viewenv M
+    ==>
+    (bir_eval_view_of_exp a_e s.bst_viewenv) <= LENGTH M
+Proof
+  metis_tac[bir_eval_view_of_exp_wf]
+QED
+
+Theorem bir_eval_exp_view_bound:
+  !l a_e s M v_addr.
+    well_formed_viewenv s.bst_viewenv M
+    /\ (SOME l, v_addr) = bir_eval_exp_view a_e s.bst_environ s.bst_viewenv
+    ==>
+    v_addr <= LENGTH M
+Proof
+  fs[bir_eval_exp_view_def, bir_eval_view_of_exp_bound]
+QED
+
+Theorem clstep_preserves_wf:
+!p cid s M prom s'.
+  well_formed cid M s
+  /\ clstep p cid s M prom s'
+==>
+  well_formed cid M s'
+Proof
+  cheat
+QED
+(* Incomplete proof for time reasons,
+   but it should be straightforward
+
+  rpt strip_tac
+  >> fs[well_formed_def]
+  >> drule_then imp_res_tac clstep_preserves_wf_fwdb
+  >> fs[clstep_cases]
+    >|
+  [ (* read *)
+    ‘v_addr <= LENGTH M’
+     by (fs[bir_eval_exp_view_def]
+         >> drule bir_eval_view_of_exp_wf
+         >> fs[])
+    >> fs[well_formed_viewenv_def]
+    >> Cases_on ‘acq /\ rel’
+    >|
+    [
+      irule_at Any mem_read_view_wf_fwdb
+      >> qexists_tac ‘l’ >> qexists_tac ‘s.bst_coh l’
+      >> gvs[]
+      >> conj_asm1_tac
+      >-
+        (‘t <= LENGTH M \/ (t = 0 /\ v = mem_default_value)’
+         by metis_tac[mem_read_some]
+         >> fs[])
+      >> rw[]
+      >> Cases_on ‘var' = var’
+      >> gvs[FLOOKUP_DEF, FLOOKUP_UPDATE]
+      >> irule mem_read_view_wf_fwdb
+      >> fs[]
+      >> qexists_tac ‘s.bst_coh l’ >> qexists_tac ‘l’
+      >> fs[]
+      ,
+      cheat
+    ]
+  , proof follows here
+  ]
+*)
+
+        
+val _ = export_theory ();
